asdf

test.fst
@@ -28,7 +28,7 @@ let rec big_endian_zero len =
   if len = 0 then ()
   else (
     let nlen = len - 1 in
-    lemma_eq_intro (slice (create len 0uy) 0 nlen) (create nlen 0uy);
+    lemma_eq_intro (slice (create len 0uy) 0 nlen) (create nlen 0uy); // TODO == ?
     big_endian_zero nlen
   )
 
@@ -80,14 +80,10 @@ private // The long form must not be all zero bytes.
 val read_length_success_lemma5: (b:Seq.seq U8.t{Seq.length b > 0}) -> Lemma
   (requires (U8.v (Seq.index b 0) > 0x80 /\ U8.v (Seq.index b 0) < 0x85 /\
              Seq.length b > U8.v (Seq.index b 0) - 0x80 /\
-             (forall i. i > 0 /\ i < Seq.length b ==> Seq.index b i = 0uy)))
+             Seq.slice b 1 (U8.v (Seq.index b 0) - 0x80 + 1) = Seq.create (U8.v (Seq.index b 0) - 0x80 + 1) 0uy))
   (ensures (not (read_length_success b)))
-let read_length_success_lemma5 b = // TODO
-   let len = U8.v (Seq.index b 0) - 0x80 + 1 in
-   assert (Seq.length b >= len /\ len >= 1);
-   Seq.lemma_eq_intro (Seq.slice b 1 len) (Seq.create (len - 1) 0uy);
-   assert (big_endian (Seq.create (len - 1) 0uy) = 0);
-   assert (big_endian (Seq.slice b 1 len) = 0)
+let read_length_success_lemma5 b =
+   assert (big_endian (Seq.slice b 1 (U8.v (Seq.index b 0) - 0x80 + 1)) = 0)
 
 //private // Success with long form means we have more than just zero bytes.
 //let read_length_success_lemma6 (b:Seq.seq U8.t{Seq.length b > 0}) : Lemma
@@ -102,7 +98,7 @@ let read_length_success_lemma5 b = // TODO
 val read_length :
   buf:buffer U8.t ->
   len:U32.t{U32.v len <= 4} ->
-  ST (r:U32.t{U32.v r < pow2 (8 * U32.v len)})
+  ST (r:U32.t{U32.v r < pow2 (8 * U32.v len)}) // TODO
   (requires (fun h -> live h buf /\ U32.v len = length buf))
   (ensures (fun h0 r h1 -> h0 == h1 /\ live h1 buf /\ U32.v r = big_endian (as_seq h0 buf)))
   (decreases (length buf))
